Request-response functions with state on the server side

src/lib/communication/DY.Lib.Communication.Core.Lemmas.fst
@@ -1,4 +1,4 @@
-module DY.Lib.Communication.API.Lemmas
+module DY.Lib.Communication.Core.Lemmas
 
 open Comparse
 open DY.Core
@@ -8,18 +8,12 @@ open DY.Lib.Crypto.Signature.Split
 open DY.Lib.State.PKI
 open DY.Lib.State.PrivateKeys
 open DY.Lib.Event.Typed
-open DY.Lib.State.Typed
 
-open DY.Lib.Communication.API.Invariants
-open DY.Lib.Communication.API
+open DY.Lib.Communication.Core
+open DY.Lib.Communication.Core.Invariants
 
 #set-options "--fuel 0 --ifuel 0 --z3cliopt 'smt.qi.eager_threshold=100'"
 
-(*** Layer Setup ***)
-
-class local_extension = {
-  local_extension_preds: comm_higher_layer_event_preds
-}
 
 (**** Confidential Send and Receive Lemmas ****)
 
@@ -44,7 +38,6 @@ let encrypt_message_proof #cinvs tr sender receiver pk_receiver nonce payload = 
 
 val send_confidential_proof:
   {|invs:protocol_invariants|} ->
-  {|lep:local_extension|} ->
   tr:trace ->
   higher_layer_preds:comm_higher_layer_event_preds ->
   keys_sess_ids:communication_keys_sess_ids ->
@@ -54,9 +47,8 @@ val send_confidential_proof:
     trace_invariant tr /\
     has_pki_invariant /\
     has_communication_layer_crypto_predicates /\
-    has_communication_layer_event_predicates lep.local_extension_preds higher_layer_preds /\
+    has_communication_layer_event_predicates higher_layer_preds /\
     higher_layer_preds.send_conf tr sender receiver payload /\
-    lep.local_extension_preds.send_conf tr sender receiver payload /\
     // We only require the payload to flow to the sender and receiver to allow
     // the sender to send a payload readable by other principals. If you want
     // the payload to be only readable by the sender and receiver, you can use
@@ -68,14 +60,13 @@ val send_confidential_proof:
     let (_, tr_out) = send_confidential keys_sess_ids sender receiver payload tr in
     trace_invariant tr_out
   ))
-let send_confidential_proof #invs #lep tr higher_layer_preds keys_sess_ids sender receiver payload =
+let send_confidential_proof #invs tr higher_layer_preds keys_sess_ids sender receiver payload =
   match send_confidential keys_sess_ids sender receiver payload tr with
   | (None, tr_out) -> ()
   | (Some _, tr_out) -> (
     let (Some pk_receiver, tr') = get_public_key sender keys_sess_ids.pki (LongTermPkEncKey comm_layer_pkenc_tag) receiver tr in
     let (nonce, tr') = mk_rand PkNonce (long_term_key_label sender) 32 tr' in
     higher_layer_preds.send_conf_later tr tr' sender receiver payload;
-    lep.local_extension_preds.send_conf_later tr tr' sender receiver payload;
     let ((), tr') = trigger_event sender (CommConfSendMsg sender receiver payload) tr' in
     assert(event_triggered tr' sender (CommConfSendMsg sender receiver payload));
     encrypt_message_proof tr' sender receiver pk_receiver nonce payload;
@@ -117,7 +108,6 @@ let decrypt_message_proof #cinvs tr receiver sk_receiver msg_encrypted =
 
 val receive_confidential_proof:
   {|invs:protocol_invariants|} ->
-  {|lep:local_extension|} ->
   tr:trace ->
   higher_layer_preds:comm_higher_layer_event_preds ->
   comm_keys_ids:communication_keys_sess_ids ->
@@ -127,7 +117,7 @@ val receive_confidential_proof:
     trace_invariant tr /\ 
     has_private_keys_invariant /\
     has_communication_layer_crypto_predicates /\
-    has_communication_layer_event_predicates lep.local_extension_preds higher_layer_preds
+    has_communication_layer_event_predicates higher_layer_preds
   )
   (ensures (
     match receive_confidential comm_keys_ids receiver msg_id tr with
@@ -137,7 +127,7 @@ val receive_confidential_proof:
       event_triggered tr_out receiver (CommConfReceiveMsg receiver payload)
     )
   ))
-let receive_confidential_proof #invs #lep tr higher_layer_preds comm_keys_ids receiver msg_id =
+let receive_confidential_proof #invs tr higher_layer_preds comm_keys_ids receiver msg_id =
   match receive_confidential comm_keys_ids receiver msg_id tr with
   | (None, tr_out) -> ()
   | (Some payload, tr_out) -> (
@@ -203,7 +193,6 @@ let sign_message_proof #cinvs tr sender receiver payload is_encrypted sk_sender 
 
 val send_authenticated_proof:
   {|invs:protocol_invariants|} ->
-  {|lep:local_extension|} ->
   tr:trace ->
   higher_layer_preds:comm_higher_layer_event_preds ->
   comm_keys_ids:communication_keys_sess_ids ->
@@ -213,7 +202,7 @@ val send_authenticated_proof:
     trace_invariant tr /\ 
     has_private_keys_invariant /\
     has_communication_layer_crypto_predicates /\
-    has_communication_layer_event_predicates lep.local_extension_preds higher_layer_preds /\
+    has_communication_layer_event_predicates higher_layer_preds /\
     higher_layer_preds.send_auth tr sender payload /\
     is_publishable tr payload
   )
@@ -221,7 +210,7 @@ val send_authenticated_proof:
     let (_, tr_out) = send_authenticated comm_keys_ids sender receiver payload tr in
     trace_invariant tr_out
   ))
-let send_authenticated_proof #invs #lep tr higher_layer_preds comm_keys_ids sender receiver payload =
+let send_authenticated_proof #invs tr higher_layer_preds comm_keys_ids sender receiver payload =
     match send_authenticated comm_keys_ids sender receiver payload tr with
     | (None, tr_out) -> ()
     | (Some _, tr_out) -> (      
@@ -297,7 +286,6 @@ let verify_message_proof #cinvs tr sender receiver msg_bytes is_encrypted vk_sen
 
 val receive_authenticated_proof:
   {|invs:protocol_invariants|} ->
-  {|lep:local_extension|} ->
   tr:trace ->
   higher_layer_preds:comm_higher_layer_event_preds ->
   comm_keys_ids:communication_keys_sess_ids ->
@@ -307,7 +295,7 @@ val receive_authenticated_proof:
     trace_invariant tr /\ 
     has_pki_invariant /\
     has_communication_layer_crypto_predicates /\
-    has_communication_layer_event_predicates lep.local_extension_preds higher_layer_preds
+    has_communication_layer_event_predicates higher_layer_preds
   )
   (ensures (
     match receive_authenticated comm_keys_ids receiver msg_id tr with
@@ -317,7 +305,7 @@ val receive_authenticated_proof:
       event_triggered tr_out receiver (CommAuthReceiveMsg sender receiver payload)
     )
   ))
-let receive_authenticated_proof #invs #lep tr higher_layer_preds comm_keys_ids receiver msg_id =
+let receive_authenticated_proof #invs tr higher_layer_preds comm_keys_ids receiver msg_id =
   match receive_authenticated comm_keys_ids receiver msg_id tr with
   | (None, tr_out) -> ()
   | (Some {sender=sender'; receiver=receiver'; payload}, tr_out) -> (
@@ -365,7 +353,6 @@ let encrypt_and_sign_message_proof #cinvs tr sender receiver payload pk_receiver
 #push-options "--z3rlimit 10"
 val send_confidential_authenticated_proof:
   {|invs:protocol_invariants|} ->
-  {|lep:local_extension|} ->
   tr:trace ->
   higher_layer_preds:comm_higher_layer_event_preds ->
   comm_keys_ids:communication_keys_sess_ids ->
@@ -376,9 +363,8 @@ val send_confidential_authenticated_proof:
     has_private_keys_invariant /\
     has_pki_invariant /\
     has_communication_layer_crypto_predicates /\
-    has_communication_layer_event_predicates lep.local_extension_preds higher_layer_preds /\
+    has_communication_layer_event_predicates higher_layer_preds /\
     higher_layer_preds.send_conf tr sender receiver payload /\
-    lep.local_extension_preds.send_conf tr sender receiver payload /\
     higher_layer_preds.send_conf_auth tr sender receiver payload /\
     is_knowable_by (join (principal_label sender) (principal_label receiver)) tr payload
   )
@@ -386,7 +372,7 @@ val send_confidential_authenticated_proof:
     let (_, tr_out) = send_confidential_authenticated comm_keys_ids sender receiver payload tr in
     trace_invariant tr_out
   ))
-let send_confidential_authenticated_proof #invs #lep tr higher_layer_preds comm_keys_ids sender receiver payload =
+let send_confidential_authenticated_proof #invs tr higher_layer_preds comm_keys_ids sender receiver payload =
   match send_confidential_authenticated comm_keys_ids sender receiver payload tr with
   | (None, tr_out) -> ()
   | (Some _, tr_out) -> (
@@ -396,7 +382,6 @@ let send_confidential_authenticated_proof #invs #lep tr higher_layer_preds comm_
     let (sign_nonce, tr') = mk_rand SigNonce (long_term_key_label sender) 32 tr' in
     
     higher_layer_preds.send_conf_later tr tr' sender receiver payload;
-    lep.local_extension_preds.send_conf_later tr tr' sender receiver payload;
     let ((), tr') = trigger_event sender (CommConfSendMsg sender receiver payload) tr' in
     assert(event_triggered tr' sender (CommConfSendMsg sender receiver payload));    
 
@@ -456,7 +441,6 @@ let verify_and_decrypt_message_proof #cinvs tr sender receiver msg_encrypted_sig
 #push-options "--z3rlimit 10"
 val receive_confidential_authenticated_proof:
   {|invs:protocol_invariants|} ->
-  {|lep:local_extension|} ->
   tr:trace ->
   higher_layer_preds:comm_higher_layer_event_preds ->
   comm_keys_ids:communication_keys_sess_ids ->
@@ -467,7 +451,7 @@ val receive_confidential_authenticated_proof:
     has_private_keys_invariant /\
     has_pki_invariant /\
     has_communication_layer_crypto_predicates /\
-    has_communication_layer_event_predicates lep.local_extension_preds higher_layer_preds
+    has_communication_layer_event_predicates higher_layer_preds
   )
   (ensures
     (
@@ -480,7 +464,7 @@ val receive_confidential_authenticated_proof:
       )
     )
   )
-let receive_confidential_authenticated_proof #invs #lep tr higher_layer_preds comm_keys_ids receiver msg_id =
+let receive_confidential_authenticated_proof #invs tr higher_layer_preds comm_keys_ids receiver msg_id =
   match receive_confidential_authenticated comm_keys_ids receiver msg_id tr with
   | (None, tr_out) -> ()
   | (Some {sender; receiver=receiver'; payload}, tr_out) -> (
@@ -494,221 +478,6 @@ let receive_confidential_authenticated_proof #invs #lep tr higher_layer_preds co
     assert(event_triggered tr receiver (CommConfAuthReceiveMsg msg.sender receiver msg.payload));
     assert(trace_invariant tr);
     assert(tr == tr_out);
-    ()
-  )
-#pop-options
-
-
-(**** Request-Response Pair Lemmas ****)
-
-val compute_request_message_proof:
-  {|crypto_invariants|} ->
-  tr:trace ->
-  client:principal -> server:principal ->
-  id:bytes -> payload:bytes -> key:bytes ->
-  Lemma
-  (requires
-    is_secret (comm_label client server) tr id /\
-    is_secret (comm_label client server) tr key /\
-    is_knowable_by (comm_label client server) tr payload
-  )
-  (ensures
-    is_knowable_by (comm_label client server) tr (compute_request_message client id payload key)
-  )
-let compute_request_message_proof #invs tr client server id payload key =
-  serialize_wf_lemma request_message (is_knowable_by (comm_label client server) tr) {client; id; payload; key};
-  ()
-
-val request_response_event_preconditions: bytes -> bytes -> comm_higher_layer_event_preds
-let request_response_event_preconditions id payload = {
-  default_comm_higher_layer_event_preds with
-  send_conf = (fun tr client server req_payload ->
-    event_triggered tr client (CommClientSendRequest client server id payload)
-  );
-}
-
-#push-options "--fuel 0 --ifuel 2"
-instance lep:local_extension = {
-  local_extension_preds = {
-    default_comm_higher_layer_event_preds with
-    send_conf = (fun tr client server req_payload ->
-      match decode_request_message req_payload with
-      | None -> False
-      | Some {id; client=client'; payload; key} -> (
-        client == client' /\
-        event_triggered tr client (CommClientSendRequest client server id payload)
-      )
-    )
-  }
-}
-#pop-options
-
-
-val send_request_proof:
-  {|protocol_invariants|} ->
-  tr:trace ->
-  comm_keys_ids:communication_keys_sess_ids ->
-  higher_layer_preds:comm_higher_layer_event_preds ->
-  client:principal -> server:principal -> payload:bytes ->
-  Lemma
-  (requires
-    trace_invariant tr /\
-    has_pki_invariant /\
-    has_communication_layer_crypto_predicates /\
-    has_communication_layer_event_predicates lep.local_extension_preds higher_layer_preds /\
-    has_communication_layer_state_predicates /\
-    higher_layer_preds.send_request tr client server payload /\
-    (forall p. higher_layer_preds.send_conf tr client server p) /\
-    is_knowable_by (comm_label client server) tr payload
-  )
-  (ensures (
-    let (_, tr_out) = send_request comm_keys_ids client server payload tr in
-    trace_invariant tr_out
-  ))
-let send_request_proof #invs tr comm_keys_ids higher_layer_preds client server payload =
-  match send_request comm_keys_ids client server payload tr with
-  | (None, tr_out) -> (
-    let (key, tr') = mk_rand (AeadKey comm_layer_aead_tag empty) (comm_label client server) 32 tr in
-    let (id, tr') = mk_rand NoUsage (comm_label client server) 32 tr' in
-    let (sid, tr') = new_session_id client tr' in
-    let ((), tr') = set_state client sid (ClientSendRequest {id; server; payload; key} <: communication_states) tr' in
-    higher_layer_preds.send_request_later tr tr' client server payload;
-    let ((), tr') = trigger_event client (CommClientSendRequest client server id payload) tr' in
-    ()
-  )
-  | (Some _, tr_out) -> (
-    let (key, tr') = mk_rand (AeadKey comm_layer_aead_tag empty) (comm_label client server) 32 tr in
-    let (id, tr') = mk_rand NoUsage (comm_label client server) 32 tr' in
-    
-    let (sid, tr') = new_session_id client tr' in
-    let ((), tr') = set_state client sid (ClientSendRequest {id; server; payload; key} <: communication_states) tr' in
-    
-    higher_layer_preds.send_request_later tr tr' client server payload;
-    assert(trace_invariant tr');
-    assert(is_knowable_by (comm_label client server) tr' payload);
-    assert(higher_layer_preds.send_request tr' client server payload);
-    let ((), tr') = trigger_event client (CommClientSendRequest client server id payload) tr' in
-    assert(trace_invariant tr');
-    assert(event_triggered tr' client (CommClientSendRequest client server id payload));
-    assert(trace_invariant tr');
-        
-    compute_request_message_proof tr' client server id payload key;
-    let req_payload = compute_request_message client id payload key in
-
-    higher_layer_preds.send_conf_later tr tr' client server req_payload;
-    assert(lep.local_extension_preds.send_conf tr' client server req_payload);
-    //lep.local_extension_preds.send_conf_later tr tr' client server req_payload;
-    assert(higher_layer_preds.send_conf tr' client server req_payload);
-    assert(lep.local_extension_preds.send_conf tr' client server req_payload);
-    send_confidential_proof #invs #lep tr' higher_layer_preds comm_keys_ids client server req_payload;
-    
-    let (Some msg_id, tr') = send_confidential comm_keys_ids client server req_payload tr' in
-    assert(tr_out == tr');
-    assert(trace_invariant tr_out);
-    ()
-  )
-
-
-val decode_request_message_proof:
-  {|crypto_invariants|} ->
-  tr:trace ->
-  server:principal -> msg_bytes:bytes ->
-  Lemma
-  (requires
-    exists client. is_knowable_by (comm_label client server) tr msg_bytes
-  )
-  (ensures (
-    match decode_request_message msg_bytes with
-    | None -> True
-    | Some {id; client=client'; payload; key} -> (
-      exists client.
-        is_knowable_by (comm_label client server) tr id /\
-        is_knowable_by (comm_label client server) tr payload /\
-        is_knowable_by (comm_label client server) tr key
-    )
-  ))
-let decode_request_message_proof #cinvs tr server msg_bytes =
-  match decode_request_message msg_bytes with
-  | None -> ()
-  | Some {id; client=client'; payload; key} -> (
-    eliminate exists client. is_knowable_by (comm_label client server) tr msg_bytes
-    returns (exists client.
-        is_knowable_by (comm_label client server) tr id /\
-        is_knowable_by (comm_label client server) tr payload /\
-        is_knowable_by (comm_label client server) tr key)
-    with _. (
-      parse_wf_lemma request_message (is_knowable_by (comm_label client server) tr) msg_bytes;
-     ()
-    )
-  )
-
-#push-options "--z3rlimit 10"
-val receive_request_proof:
-  {|protocol_invariants|} ->
-  tr:trace ->
-  comm_keys_ids:communication_keys_sess_ids ->
-  higher_layer_preds:comm_higher_layer_event_preds ->
-  server:principal -> msg_id:timestamp ->
-  Lemma
-  (requires
-    trace_invariant tr /\
-    has_private_keys_invariant /\
-    has_pki_invariant /\
-    has_communication_layer_crypto_predicates /\
-    has_communication_layer_event_predicates lep.local_extension_preds higher_layer_preds /\
-    has_communication_layer_state_predicates
-  )
-  (ensures (
-    match receive_request comm_keys_ids server msg_id tr with
-    | (None, tr_out) -> trace_invariant tr_out
-    | (Some (sid, payload), tr_out) -> (
-      trace_invariant tr_out /\
-      (exists client. is_knowable_by (comm_label client server) tr_out payload)
-    )
-  ))
-let receive_request_proof #invs tr comm_keys_ids higher_layer_preds server msg_id =
-  match receive_request comm_keys_ids server msg_id tr with
-  | (None, tr_out) -> ()
-  | (Some (sid, payload), tr_out) -> (
-    receive_confidential_proof #invs #lep tr higher_layer_preds comm_keys_ids server msg_id;
-    let (Some req_msg_bytes, tr) = receive_confidential comm_keys_ids server msg_id tr in
-    
-    assert(exists client.
-      event_triggered tr client (CommConfSendMsg client server req_msg_bytes) \/
-          is_publishable tr req_msg_bytes
-    );
-    assert(exists client.
-      lep.local_extension_preds.send_conf tr client server req_msg_bytes \/
-          is_publishable tr req_msg_bytes
-    );
-
-    decode_request_message_proof tr server req_msg_bytes;
-    let Some req_msg = decode_request_message req_msg_bytes in
-
-    FStar.Classical.move_requires (parse_wf_lemma request_message (is_publishable tr)) req_msg_bytes;
-    assert(exists client.
-      event_triggered tr client (CommClientSendRequest client server req_msg.id req_msg.payload) \/
-        is_publishable tr req_msg.payload
-    );
-
-    assert(exists client.
-      is_knowable_by (comm_label client server) tr req_msg.id /\
-      is_knowable_by (comm_label client server) tr req_msg.payload /\
-      is_knowable_by (comm_label client server) tr req_msg.key
-    );
-    
-   
-    let (sid, tr) = new_session_id server tr in
-    assert(trace_invariant tr);
-    let ((), tr) = set_state server sid (ServerReceiveRequest {id=req_msg.id; client=req_msg.client; payload=req_msg.payload; key=req_msg.key} <: communication_states) tr in
-    assert(trace_invariant tr);
-
-    let ((), tr) = trigger_event server (CommServerReceiveRequest server req_msg.id req_msg.payload) tr in
-    assert(trace_invariant tr);
-    assert(event_triggered tr server (CommServerReceiveRequest server req_msg.id req_msg.payload));
-    
-    assert(tr == tr_out);
-    assert(trace_invariant tr_out);
     ()
   )
 #pop-options
