src/lib/communication/DY.Lib.Communication.RequestResponse.fst
@@ -1,0 +1,243 @@
+module DY.Lib.Communication.RequestResponse
+
+open Comparse
+open DY.Core
+open DY.Lib.State.PKI
+open DY.Lib.State.PrivateKeys
+open DY.Lib.Event.Typed
+open DY.Lib.State.Typed
+
+open DY.Lib.Communication.Core
+
+#set-options "--fuel 0 --ifuel 0 --z3cliopt 'smt.qi.eager_threshold=100'"
+
+(*** Messages ***)
+
+[@@with_bytes bytes]
+type request_message = {
+  id:bytes;
+  client:principal;
+  payload:bytes;
+  key:bytes
+}
+
+%splice [ps_request_message] (gen_parser (`request_message))
+%splice [ps_request_message_is_well_formed] (gen_is_well_formed_lemma (`request_message))
+
+instance parseable_serializeable_bytes_request_message: parseable_serializeable bytes request_message
+  = mk_parseable_serializeable ps_request_message
+
+[@@with_bytes bytes]
+type response_message = {
+  id:bytes;
+  payload:bytes
+}
+
+%splice [ps_response_message] (gen_parser (`response_message))
+%splice [ps_response_message_is_well_formed] (gen_is_well_formed_lemma (`response_message))
+
+instance parseable_serializeable_bytes_response_message: parseable_serializeable bytes response_message
+  = mk_parseable_serializeable ps_response_message
+
+[@@with_bytes bytes]
+type response_envelope = {
+  nonce:bytes;
+  ciphertext:bytes
+}
+
+%splice [ps_response_envelope] (gen_parser (`response_envelope))
+%splice [ps_response_envelope_is_well_formed] (gen_is_well_formed_lemma (`response_envelope))
+
+instance parseable_serializeable_bytes_response_envelope: parseable_serializeable bytes response_envelope
+  = mk_parseable_serializeable ps_response_envelope
+
+[@@with_bytes bytes]
+type authenticated_data = {
+  client:principal;
+  server:principal
+}
+
+%splice [ps_authenticated_data] (gen_parser (`authenticated_data))
+%splice [ps_authenticated_data_is_well_formed] (gen_is_well_formed_lemma (`authenticated_data))
+
+instance parseable_serializeable_bytes_authenticated_data: parseable_serializeable bytes authenticated_data
+  = mk_parseable_serializeable ps_authenticated_data
+
+
+[@@with_bytes bytes]
+type request_meta_data = {
+  id:bytes;
+  key:bytes
+}
+
+
+(*** States ***)
+
+[@@with_bytes bytes]
+type client_send_request = {
+  id:bytes;
+  server:principal;
+  payload:bytes;
+  key:bytes
+}
+
+%splice [ps_client_send_request] (gen_parser (`client_send_request))
+%splice [ps_client_send_request_is_well_formed] (gen_is_well_formed_lemma (`client_send_request))
+
+[@@with_bytes bytes]
+type server_receive_request = {
+  id:bytes;
+  client:principal;
+  payload:bytes;
+  key:bytes
+}
+
+%splice [ps_server_receive_request] (gen_parser (`server_receive_request))
+%splice [ps_server_receive_request_is_well_formed] (gen_is_well_formed_lemma (`server_receive_request))
+
+[@@with_bytes bytes]
+type client_receive_response = {
+  id:bytes;
+  server:principal;
+  payload:bytes;
+  key:bytes
+}
+
+%splice [ps_client_receive_response] (gen_parser (`client_receive_response))
+%splice [ps_client_receive_response_is_well_formed] (gen_is_well_formed_lemma (`client_receive_response))
+
+[@@with_bytes bytes]
+type communication_states =
+  | ClientSendRequest: client_send_request -> communication_states
+  | ServerReceiveRequest: server_receive_request -> communication_states
+  | ClientReceiveResponse: client_receive_response -> communication_states
+
+#push-options "--ifuel 1"
+%splice [ps_communication_states] (gen_parser (`communication_states))
+%splice [ps_communication_states_is_well_formed] (gen_is_well_formed_lemma (`communication_states))
+#pop-options
+
+instance parseable_serializeable_bytes_communication_states: parseable_serializeable bytes communication_states
+  = mk_parseable_serializeable ps_communication_states
+
+instance local_state_communication_layer_session: local_state communication_states = {
+  tag = "DY.Lib.Communication.State.RequestResponse";
+  format = parseable_serializeable_bytes_communication_states;
+}
+
+[@@with_bytes bytes]
+type communication_reqres_event =
+  | CommClientSendRequest: client:principal -> server:principal -> id:bytes -> payload:bytes -> key:bytes -> communication_reqres_event
+  | CommServerReceiveRequest: client:principal -> server:principal -> id:bytes -> payload:bytes -> key:bytes -> communication_reqres_event
+  | CommServerSendResponse: client:principal -> server:principal -> id:bytes -> payload:bytes -> communication_reqres_event
+  | CommClientReceiveResponse: client:principal -> server:principal -> id:bytes -> payload:bytes -> key:bytes -> communication_reqres_event
+
+#push-options "--ifuel 1"
+%splice [ps_communication_reqres_event] (gen_parser (`communication_reqres_event))
+%splice [ps_communication_reqres_event_is_well_formed] (gen_is_well_formed_lemma (`communication_reqres_event))
+#pop-options
+
+instance event_communication_reqres_event: event communication_reqres_event = {
+  tag = "DY.Lib.Communication.Event.RequestResponse";
+  format = mk_parseable_serializeable ps_communication_reqres_event;
+}
+
+(*** Layer Setup ***)
+
+val comm_layer_aead_tag: string
+let comm_layer_aead_tag = "DY.Lib.Communication.Aead.Key"
+
+(*** API ***)
+
+val compute_request_message: principal -> bytes -> bytes -> bytes -> bytes
+let compute_request_message client id payload key =
+  let req:request_message = {client; id; payload; key} in
+  serialize request_message req
+
+val send_request:
+  communication_keys_sess_ids ->
+  principal -> principal -> bytes ->
+  traceful (option (state_id & timestamp))
+let send_request comm_keys_ids client server payload =
+  let* key = mk_rand (AeadKey comm_layer_aead_tag empty) (comm_label client server) 32 in
+  let* id = mk_rand NoUsage (join (principal_label client) (principal_label server)) 32 in
+  
+  let* sid = new_session_id client in
+  set_state client sid (ClientSendRequest {id; server; payload; key} <: communication_states);*
+  trigger_event client (CommClientSendRequest client server id payload key);*
+  
+  let* req_payload = return (compute_request_message client id payload key) in
+  let*? msg_id = send_confidential comm_keys_ids client server req_payload in
+  return (Some (sid, msg_id))
+
+val decode_request_message: bytes -> option request_message
+let decode_request_message msg_bytes =
+  parse request_message msg_bytes
+
+val receive_request:
+  communication_keys_sess_ids ->
+  principal -> timestamp ->
+  traceful (option (state_id & bytes & (FStar.Ghost.erased principal) & (FStar.Ghost.erased bytes) & (FStar.Ghost.erased bytes)))
+let receive_request comm_keys_ids server msg_id =
+  let*? req_msg_bytes = receive_confidential comm_keys_ids server msg_id in
+  let*? req_msg:request_message = return (decode_request_message req_msg_bytes) in  
+  trigger_event server (CommServerReceiveRequest req_msg.client server req_msg.id req_msg.payload req_msg.key);*
+  let* sid = new_session_id server in
+  set_state server sid (ServerReceiveRequest {id=req_msg.id; client=req_msg.client; payload=req_msg.payload; key=req_msg.key} <: communication_states);*
+  let* tr = get_trace in
+  return (Some (sid, req_msg.payload, FStar.Ghost.hide req_msg.client, FStar.Ghost.hide req_msg.id, FStar.Ghost.hide req_msg.key))
+
+val mk_comm_layer_response_nonce: principal -> state_id -> usage -> traceful (option bytes)
+let mk_comm_layer_response_nonce server sid usg =
+  let*? state = get_state server sid in
+  guard_tr (ServerReceiveRequest? state);*?
+  let ServerReceiveRequest srr = state in
+  let* tr = get_trace in
+  let* nonce = mk_rand usg (get_label #default_crypto_usages tr srr.key) 32 in
+  return (Some nonce)
+
+val compute_response_message: principal -> principal -> bytes -> bytes -> bytes -> bytes -> bytes
+let compute_response_message client server key nonce id payload =
+  let res:response_message = {id; payload} in
+  let res_bytes = serialize response_message res in
+  let ad:authenticated_data = {client; server} in
+  let ad_bytes = serialize authenticated_data ad in
+  let ciphertext = aead_enc key nonce res_bytes ad_bytes in
+  serialize response_envelope {nonce; ciphertext}
+
+val send_response:
+  communication_keys_sess_ids ->
+  principal -> state_id -> bytes -> traceful (option timestamp)
+let send_response comm_keys_ids server sid payload =
+  let*? state = get_state server sid in
+  guard_tr (ServerReceiveRequest? state);*?
+  let ServerReceiveRequest srr = state in
+  trigger_event server (CommServerSendResponse srr.client server srr.id payload);*
+  let* nonce = mk_rand NoUsage public 32 in
+  let resp_msg = compute_response_message srr.client server srr.key nonce srr.id payload in
+  let* msg_id = send_msg resp_msg in
+  return (Some msg_id)
+
+val decode_response_message: principal -> principal -> bytes -> bytes -> bytes -> option bytes
+let decode_response_message client server key id msg_bytes =
+  let? resp_env:response_envelope = parse response_envelope msg_bytes in
+  let ad:authenticated_data = {client; server} in
+  let ad_bytes = serialize authenticated_data ad in
+  let? resp_bytes = aead_dec key resp_env.nonce resp_env.ciphertext ad_bytes in
+  let? resp = parse response_message resp_bytes in
+  guard (id = resp.id);?
+  Some resp.payload
+
+val receive_response:
+  communication_keys_sess_ids ->
+  principal -> state_id -> timestamp ->
+  traceful (option bytes)
+let receive_response comm_keys_ids client sid msg_id =
+  let*? state = get_state client sid in
+  guard_tr (ClientSendRequest? state);*?
+  let ClientSendRequest csr = state in
+  let*? resp_msg_bytes = recv_msg msg_id in
+  let*? payload = return (decode_response_message client csr.server csr.key csr.id resp_msg_bytes) in
+  set_state client sid (ClientReceiveResponse {id=csr.id; server=csr.server; payload; key=csr.key} <: communication_states);*
+  trigger_event client (CommClientReceiveResponse client csr.server csr.id payload csr.key);*
+  return (Some payload)
